\begin{answer} \\

$$
J(\beta)=0\;\Longleftrightarrow\;X\beta=\vec y .
$$

\(\textbf{Sufficiency }\Longleftarrow{}\)
$$
\beta=X^{\top}(XX^{\top})^{-1}\vec y+\zeta,\qquad X\zeta=0 .
$$
$$
X\beta
=XX^{\top}(XX^{\top})^{-1}\vec y+X\zeta
=\vec y+0
=\vec y,
$$
so $J(\beta)=0$.

\(\textbf{Necessity }\Longrightarrow{}\)

zero cost: $X\beta=\vec y$.
$$
     \beta = X^\top(XX^\top)^{-1}y + \bigl(I - X^\top(XX^\top)^{-1}X\bigr)\beta .
$$
The projector $I - X^\top(XX^\top)^{-1}X$ sends any vector to the null-space of $X$, i.e.,
$$
\boxed{\;\zeta \;=\; \bigl(I - X^{\top}(XX^{\top})^{-1}X\bigr)\beta\;}
$$
so that
$$
\beta
=X^{\top}(XX^{\top})^{-1}\vec y+\zeta .
$$

(check orthogonality)

$$
X\zeta
=X\beta-XX^{\top}(XX^{\top})^{-1}X\beta
=\vec y-\vec y
=0 .
$$

Hence

$$
\boxed{\;
\beta\text{ minimizes }J \iff
\beta=X^{\top}(XX^{\top})^{-1}\vec y+\zeta,\;X\zeta=0
\;}
$$
\end{answer}
