\begin{answer}
let

$$
\rho=X^{\top}(XX^{\top})^{-1}\vec y,
\qquad
\beta=\rho+\zeta,
\qquad
X\zeta=0 .
$$
$$
\|\beta\|_{2}^{2}
=(\rho+\zeta)^{\!\top}(\rho+\zeta)
=\rho^{\top}\rho+2\rho^{\top}\zeta+\zeta^{\top}\zeta .
$$

$$
\rho^{\top}\zeta
=\bigl(X^{\top}(XX^{\top})^{-1}\vec y\bigr)^{\!\top}\zeta
=\vec y^{\top}(XX^{\top})^{-1}X\zeta
=\vec y^{\top}(XX^{\top})^{-1}\,0
=0 .
$$

$$
\Longrightarrow\;
\|\beta\|_{2}^{2}
=\|\rho\|_{2}^{2}+\|\zeta\|_{2}^{2}
\;\ge\;\|\rho\|_{2}^{2}.
$$
so
$$
\boxed{\;\|\rho\|_{2}\le\|\beta\|_{2}\;}
$$
\end{answer}