\begin{answer}
$$
J(\theta)=\frac12\sum_{i=1}^{n}\bigl(\theta^{\top}\hat{x}^{(i)}-y^{(i)}\bigr)^2,
\qquad\text{where } \hat{x}^{(i)}=\bigl[1,\;x^{(i)},\;(x^{(i)})^2,\;(x^{(i)})^3\bigr]^{\!\top}.
$$
$$
=\frac12\bigl(\hat{X}\theta-y\bigr)^{\!\top}\bigl(\hat{X}\theta-y\bigr)
$$

$$
\nabla_{\theta}J(\theta)=\frac12\cdot2\,\hat{X}^{\top}\bigl(\hat{X}\theta-y\bigr)=\hat{X}^{\top}\bigl(\hat{X}\theta-y\bigr)
$$

$$
\boxed{\;
\theta^{[t]} \;=\; \theta^{[t-1]} \;-\;\alpha\,\hat{X}^{\top}\bigl(\hat{X}\,\theta^{[t-1]} - y\bigr)
\;}
$$

\end{answer}
