
\begin{answer}
$$
J_{\lambda}(\beta)
=\frac12\lVert X\beta-\vec y\rVert_{2}^{2}
\;+\;\frac{\lambda}{2}\lVert\beta\rVert_{2}^{2}
$$
$$
\text{since }\hat{\beta}_{\lambda}\;=\;\arg\min_{\beta\in\mathbb{R}^{d}} J_{\lambda}(\beta),
$$
$$
\nabla_{\beta}J_{\lambda}(\beta)
= X^{\top}(X\beta-\vec y)+\lambda\beta=0
$$

$$
\Longrightarrow\;\bigl(X^{\top}X+\lambda I_{d\times d}\bigr)\,\beta
= X^{\top}\vec y.
$$

$$
z^{\top}\bigl(X^{\top}X+\lambda I\bigr)z
=\lVert Xz\rVert_{2}^{2}+\lambda\lVert z\rVert_{2}^{2}>0
\;\;(\forall z\ne0,\;\lambda>0)
\;\Longrightarrow\;
X^{\top}X+\lambda I \text{ invertible}.
$$

$$
\boxed{\;
\hat{\beta}_{\lambda}=
\bigl(X^{\top}X+\lambda I_{d\times d}\bigr)^{-1}\,X^{\top}\vec y
\;}
$$
\end{answer}
